

Linear Algebra Problems

Tristan Chaang

November 16, 2020

1 Similar Matrices

1. Let A and X be $n \times n$ invertible matrices such that $XAX^{-1} = A^2$. Prove that there exists a positive integer m such that all the eigenvalues of A are m -th roots of unity.

Solution:

Recall that similar matrices have the same eigenvalues. Let λ be an eigenvalue of A , then

$$Av = \lambda v \Rightarrow A^2v = \lambda Av = \lambda^2v$$

hence λ^2 is an eigenvalue of $A^2 = XAX^{-1} \Rightarrow \lambda^2$ is an eigenvalue of A . Inductively, λ^{2^n} is an eigenvalue of A for any $n \in \mathbb{N}$. Since there are finitely many eigenvalues, $\lambda^i = \lambda^j$ for some $i \neq j$, hence λ is a root of unity, say $\lambda^{f(\lambda)} = 1$. Repeat for all eigenvalues of A and take m as the LCM of all $f(\lambda)$. \square

2 Olympiad

2. Let A_1, A_2, \dots, A_{n+1} be non-empty subsets of $\{1, 2, \dots, n\}$. Prove that there exists nonempty disjoint subsets $I, J \in \{1, 2, \dots, n+1\}$ such that

$$\bigcup_{k \in I} A_k = \bigcup_{k \in J} A_k$$

Solution:

Let v_i be the incidence vector of A_i . Since v_1, \dots, v_{n+1} are linearly dependent in n -dimensions, there exists $c_1, \dots, c_{n+1} \in \mathbb{R}$, not all zero, such that

$$c_1v_1 + \dots + c_{n+1}v_{n+1} = 0.$$

Let $I = \{k : c_k > 0\}$ and $J = \{k : c_k < 0\}$. Then

$$\begin{aligned} \sum_{k \in I} |c_k|v_k &= \sum_{k \in J} |c_k|v_k \\ \therefore \bigcup_{k \in I} A_k &= \bigcup_{k \in J} A_k \end{aligned}$$

3. Let A_1, A_2, \dots, A_{n+2} be non-empty subsets of $\{1, 2, \dots, n\}$. Prove that there exists nonempty disjoint subsets $I, J \in \{1, 2, \dots, n+2\}$ such that

$$\bigcup_{k \in I} A_k = \bigcup_{k \in J} A_k \quad \text{and} \quad \bigcap_{k \in I} A_k = \bigcap_{k \in J} A_k$$

Solution:

Let v_i be the incidence vector of A_i .

Lemma. There exists $c_1, \dots, c_{n+2} \in \mathbb{R}$, not all zero, such that

$$c_1 v_1 + \dots + c_{n+2} v_{n+2} = 0 \quad \text{and} \quad c_1 + \dots + c_{n+2} = 0.$$

Proof. Assume the contrary. Let $p_1, \dots, p_{n+1} \in \mathbb{R}$, not all zero, such that

$$\begin{cases} p_1 v_1 + \dots + p_{n+1} v_{n+1} = 0 \\ p_1 + \dots + p_{n+1} = 1. \end{cases}$$

Then there must exist a positive p_i , WLOG $p_1 > 0$. Now let $q_2, \dots, q_{n+2} \in \mathbb{R}$, not all zero, such that

$$\begin{cases} q_2 v_2 + \dots + q_{n+2} v_{n+2} = 0 \\ q_2 + \dots + q_{n+2} = 1. \end{cases}$$

By subtraction we have

$$p_1 v_1 + (p_2 - q_2) v_2 + \dots + (p_{n+1} - q_{n+1}) v_{n+1} + (-q_{n+2}) v_{n+2} = 0$$

and hence we can let $c_1 = p_1 \neq 0$, $c_{n+2} = -q_{n+2}$, and $c_i = p_i - q_i$ ($i = 2, \dots, n+1$). \square

Let $I = \{k : c_k > 0\}$ and $J = \{k : c_k < 0\}$. Then

$$\begin{aligned} \sum_{k \in I} |c_k| v_k &= \sum_{k \in J} |c_k| v_k \\ \therefore \bigcup_{k \in I} A_k &= \bigcup_{k \in J} A_k \end{aligned}$$

We now prove the second property. Assume $x \in \bigcap_{k \in I} A_k$, so the x -th component of all v_k ($k \in I$) is 1.

Then the x -th component of $\sum_{k \in I} |c_k| v_k$ is equal to $\sum_{k \in I} |c_k| = \sum_{k \in J} |c_k|$. However, in the x -th component in

$\sum_{k \in I} |c_k| v_k$, the sum $\sum_{k \in J} |c_k|$ is maximal and can only be achieved when the x -th component of all v_k ($k \in J$)

is 1, hence $x \in \bigcap_{k \in J} A_k$. Similarly, $x \in \bigcap_{k \in J} A_k \Rightarrow x \in \bigcap_{k \in I} A_k$. Therefore, $\bigcap_{k \in I} A_k = \bigcap_{k \in J} A_k$. \square

4. Compute the determinant of

$$\mathbf{M} = \begin{pmatrix} a_1^2 + k & a_1a_2 & a_1a_3 & \cdots & a_1a_n \\ a_2a_1 & a_2^2 + k & a_2a_3 & \cdots & a_2a_n \\ a_3a_1 & a_3a_2 & a_3^2 + k & \cdots & a_3a_n \\ \vdots & \vdots & \vdots & \ddots & \vdots \\ a_na_1 & a_na_2 & a_na_3 & \cdots & a_n^2 + k \end{pmatrix}$$

Solution 1:

Note that $\text{rank}(\mathbf{M} - k\mathbf{I}) = 1 \Rightarrow \text{null}(\mathbf{M} - k\mathbf{I}) = n - 1$. Therefore there exists $n - 1$ mutually orthonormal vectors in the null space of $\mathbf{M} - k\mathbf{I}$, i.e. there are $n - 1$ mutually orthonormal eigenvectors $\mathbf{v}_1, \mathbf{v}_2, \dots, \mathbf{v}_{n-1}$ of \mathbf{M} with eigenvalue k . Now we see

$$\mathbf{v} = (a_1 \ a_2 \ \cdots \ a_n)^T \Rightarrow \mathbf{M}\mathbf{v} = (a_1^2 + a_2^2 + \cdots + a_n^2 + k)\mathbf{v}$$

and hence \mathbf{v} is another eigenvector of \mathbf{M} , with eigenvalue $h = a_1^2 + a_2^2 + \cdots + a_n^2 + k$. We claim that \mathbf{v} is orthogonal to any of the \mathbf{v}_i ($i = 1, \dots, n - 1$). Indeed,

$$k\mathbf{v}^T\mathbf{v}_i = \mathbf{v}^T\mathbf{M}\mathbf{v}_i = (\mathbf{M}^T\mathbf{v})^T\mathbf{v}_i = (\mathbf{M}\mathbf{v})^T\mathbf{v}_i = h\mathbf{v}^T\mathbf{v}_i \Rightarrow \mathbf{v}^T\mathbf{v}_i = 0.$$

Therefore $\hat{\mathbf{v}}, \mathbf{v}_1, \mathbf{v}_2, \dots, \mathbf{v}_{n-1}$ are mutually orthonormal eigenvectors of \mathbf{M} ! In that case,

$$\mathbf{Q} = (\hat{\mathbf{v}} \ \mathbf{v}_1 \ \mathbf{v}_2 \ \cdots \ \mathbf{v}_{n-1}) \Rightarrow \mathbf{M} = \mathbf{Q} \begin{pmatrix} h & 0 & 0 & \cdots & 0 \\ 0 & k & 0 & \cdots & 0 \\ 0 & 0 & k & \cdots & 0 \\ \vdots & \vdots & \vdots & \ddots & \vdots \\ 0 & 0 & 0 & \cdots & k \end{pmatrix} \mathbf{Q}^{-1}$$

which implies $\det(M) = k^{n-1}h = k^{n-1}(a_1^2 + a_2^2 + \cdots + a_n^2 + k)$.

Solution 2:

We prove by simple induction,

$$\begin{aligned} \det(M) &= \begin{vmatrix} a_1^2 & a_1a_2 & a_1a_3 & \cdots & a_1a_n \\ a_2a_1 & a_2^2 + k & a_2a_3 & \cdots & a_2a_n \\ a_3a_1 & a_3a_2 & a_3^2 + k & \cdots & a_3a_n \\ \vdots & \vdots & \vdots & \ddots & \vdots \\ a_na_1 & a_na_2 & a_na_3 & \cdots & a_n^2 + k \end{vmatrix} + \begin{vmatrix} k & 0 & 0 & \cdots & 0 \\ a_2a_1 & a_2^2 + k & a_2a_3 & \cdots & a_2a_n \\ a_3a_1 & a_3a_2 & a_3^2 + k & \cdots & a_3a_n \\ \vdots & \vdots & \vdots & \ddots & \vdots \\ a_na_1 & a_na_2 & a_na_3 & \cdots & a_n^2 + k \end{vmatrix} \\ &= \begin{vmatrix} a_1^2 & a_1a_2 & a_1a_3 & \cdots & a_1a_n \\ 0 & k & 0 & \cdots & 0 \\ 0 & 0 & k & \cdots & 0 \\ \vdots & \vdots & \vdots & \ddots & \vdots \\ 0 & 0 & 0 & \cdots & k \end{vmatrix} + k \begin{vmatrix} a_2^2 + k & a_2a_3 & \cdots & a_2a_n \\ a_3a_2 & a_3^2 + k & \cdots & a_3a_n \\ \vdots & \vdots & \ddots & \vdots \\ a_na_2 & a_na_3 & \cdots & a_n^2 + k \end{vmatrix} \\ &= a_1^2k^{n-1} + k^{n-1}(a_2^2 + \cdots + a_n^2) = k^{n-1}(a_1^2 + a_2^2 + \cdots + a_n^2 + k). \end{aligned}$$

5. Let \mathbf{A} and \mathbf{B} be equally sized matrices. Prove that $\text{rank}(\mathbf{A}) + \text{rank}(\mathbf{B}) \geq \text{rank}(\mathbf{A} + \mathbf{B})$.

Solution:

Let $r = \text{rank}(\mathbf{A})$, $s = \text{rank}(\mathbf{B})$, $t = \text{rank}(\mathbf{A} + \mathbf{B})$. Pick u_1, \dots, u_r as a basis of $C(\mathbf{A})$ whereas v_1, \dots, v_s as a basis of $C(\mathbf{B})$. Let \vec{x} be any vector in $C(\mathbf{A} + \mathbf{B})$,

$$\begin{aligned}\vec{x} &= (\mathbf{A} + \mathbf{B})\vec{y} \\ &= \mathbf{A}\vec{y} + \mathbf{B}\vec{y}\end{aligned}$$

for some vector \vec{y} . Since $\mathbf{A}\vec{y}$ and $\mathbf{B}\vec{y}$ are in $C(\mathbf{A})$ and $C(\mathbf{B})$ respectively, they can be expressed as a linear combination of u_i ($1 \leq i \leq r$) and v_i ($1 \leq i \leq s$) respectively.

Therefore **any vector in $C(\mathbf{A} + \mathbf{B})$ can be expressed as a linear combination of $u_1, \dots, u_r, v_1, \dots, v_s$, which is at most $r + s$ vectors (some of them might be equal).**

Choose a basis B of the space spanned by $S = \{u_1, \dots, u_r, v_1, \dots, v_s\}$. Since any vector in $C(\mathbf{A} + \mathbf{B})$ can be written as a linear combination of B which is linearly independent, we conclude that B is also a basis of $C(\mathbf{A} + \mathbf{B})$. Because $B \subseteq S$,

$$t = |B| \leq |S| = r + s$$

which completes the proof. □